Added an invariant asserted at every step to the abstract program logics

src/theory/bin_hoare_logic/bin_hoare_logicScript.sml
@@ -15,24 +15,26 @@ val _ = Datatype `bin_model_t =
      * states is OK, through using a set of labels for which
      * execution must halt if reached, meaning they cannot be
      * touched in any intermediate step *)
-    weak : 'a -> ('b -> bool) -> 'a -> bool;
+    weak : 'a -> ('a -> bool) -> ('b -> bool) -> 'a -> bool;
     (* A function to obtain the program counter from a state *)
     pc : 'a -> 'b
    |>`;
 
 val weak_model_def = Define `
   weak_model m =
-    !ms ls ms'.
-      (m.weak ms ls ms') =
+    !ms invar ls ms'.
+      (m.weak ms invar ls ms') =
         ?n.
           ((n > 0) /\
            (FUNPOW_OPT m.trs n ms = SOME ms') /\
+           (invar ms) /\
            ((m.pc ms') IN ls)
           ) /\
           !n'.
             (((n' < n) /\ (n' > 0)) ==>
             ?ms''.
               (FUNPOW_OPT m.trs n' ms = SOME ms'') /\
+              (invar ms'') /\
               (~((m.pc ms'') IN ls))
             )`;
 
@@ -40,9 +42,9 @@ val weak_model_def = Define `
 val weak_comp_thm = prove(``
   !m.
   weak_model m ==>
-  !ms ls1 ls2 ms' ms''.
-  (m.weak ms (ls1 UNION ls2) ms') ==> (~((m.pc ms') IN ls2)) ==>
-  (m.weak ms' ls2 ms'') ==> (m.weak ms ls2 ms'')``,
+  !ms invar ls1 ls2 ms' ms''.
+  (m.weak ms invar (ls1 UNION ls2) ms') ==> (~((m.pc ms') IN ls2)) ==>
+  (m.weak ms' invar ls2 ms'') ==> (m.weak ms invar ls2 ms'')``,
 
 REPEAT STRIP_TAC >>
 REV_FULL_SIMP_TAC std_ss [weak_model_def] >>
@@ -67,11 +69,10 @@ REV_FULL_SIMP_TAC arith_ss []
 val weak_unique_thm = prove(``
   !m.
   (weak_model m) ==>
-  !ms ls ms' ms''.
-  (m.weak ms ls ms') ==>
-  (m.weak ms ls ms'') ==>
-  (ms' = ms'')
-``,
+  !ms invar1 invar2 ls ms' ms''.
+  (m.weak ms invar1 ls ms') ==>
+  (m.weak ms invar2 ls ms'') ==>
+  (ms' = ms'')``,
 
 REPEAT STRIP_TAC >>
 REV_FULL_SIMP_TAC std_ss [weak_model_def] >>
@@ -90,10 +91,10 @@ FULL_SIMP_TAC arith_ss []
 val weak_union_thm = prove(``
   !m.
   weak_model m ==>
-  !ms ls1 ls2 ms'.
-  (m.weak ms (ls1 UNION ls2) ms') ==>
+  !ms invar ls1 ls2 ms'.
+  (m.weak ms invar (ls1 UNION ls2) ms') ==>
   (~ ((m.pc ms') IN ls1)) ==>
-  (m.weak ms ls2 ms')``,
+  (m.weak ms invar ls2 ms')``,
 
 REPEAT STRIP_TAC >>
 REV_FULL_SIMP_TAC std_ss [weak_model_def] >>
@@ -104,10 +105,10 @@ METIS_TAC [pred_setTheory.IN_UNION]
 val weak_union2_thm = prove(``
   !m.
   weak_model m ==>
-  !ms ls1 ls2 ms'.
-  (m.weak ms (ls1 UNION ls2) ms') ==>
+  !ms invar ls1 ls2 ms'.
+  (m.weak ms invar (ls1 UNION ls2) ms') ==>
   (((m.pc ms') IN ls2)) ==>
-  (m.weak ms ls2 ms')``,
+  (m.weak ms invar ls2 ms')``,
 
 REPEAT STRIP_TAC >>
 REV_FULL_SIMP_TAC std_ss [weak_model_def] >>
@@ -118,10 +119,10 @@ METIS_TAC [pred_setTheory.IN_UNION]
 val weak_union_singleton_thm = prove(``
   !m.
   weak_model m ==>
-  !ms l1 ls2 ms'.
-  (m.weak ms ({l1} UNION ls2) ms') ==>
+  !ms invar l1 ls2 ms'.
+  (m.weak ms invar ({l1} UNION ls2) ms') ==>
   ((m.pc ms') <> l1) ==>
-  (m.weak ms ls2 ms')``,
+  (m.weak ms invar ls2 ms')``,
 
 METIS_TAC [weak_union_thm, pred_setTheory.IN_SING]
 );
@@ -129,8 +130,8 @@ METIS_TAC [weak_union_thm, pred_setTheory.IN_SING]
 val weak_singleton_pc_thm = prove(``
   !m.
   weak_model m ==>
-  !ms e ms'.
-  (m.weak ms {e} ms') ==> ((m.pc ms') = e)``,
+  !ms invar e ms'.
+  (m.weak ms invar {e} ms') ==> ((m.pc ms') = e)``,
 
 METIS_TAC [weak_model_def, pred_setTheory.IN_SING]
 );
@@ -139,8 +140,8 @@ METIS_TAC [weak_model_def, pred_setTheory.IN_SING]
 val weak_pc_in_thm = prove(``
   !m.
   weak_model m ==>
-  !ms ls ms'.
-  (m.weak ms ls ms') ==> ((m.pc ms') IN ls)``,
+  !ms invar ls ms'.
+  (m.weak ms invar ls ms') ==> ((m.pc ms') IN ls)``,
 
 METIS_TAC [weak_model_def]
 );
@@ -148,10 +149,10 @@ METIS_TAC [weak_model_def]
 val weak_union_pc_not_in_thm = store_thm("weak_union_pc_not_in_thm",
   ``!m.
     weak_model m ==>
-    !ms e ls1 ls2 ms'.
-    (m.weak ms (ls1 UNION ls2) ms') ==>
+    !ms invar e ls1 ls2 ms'.
+    (m.weak ms invar (ls1 UNION ls2) ms') ==>
     (~((m.pc ms') IN ls2)) ==>
-    (m.weak ms ls1 ms')``,
+    (m.weak ms invar ls1 ms')``,
 
 REPEAT STRIP_TAC >>
 REV_FULL_SIMP_TAC std_ss [weak_model_def] >>
@@ -159,56 +160,135 @@ METIS_TAC [pred_setTheory.IN_UNION]
 );
 
 
+val weak_invar_weak_thm = prove(``
+  !m.
+  weak_model m ==>
+  !ms invar1 invar2 ls ms'.
+  (!ms. (invar1 ms) ==> (invar2 ms)) ==>
+  (m.weak ms invar1 ls ms') ==>
+  (m.weak ms invar2 ls ms')``,
+
+REPEAT STRIP_TAC >>
+REV_FULL_SIMP_TAC std_ss [weak_model_def] >>
+Q.EXISTS_TAC `n` >>
+FULL_SIMP_TAC std_ss [] >>
+REPEAT STRIP_TAC >>
+QSPECL_X_ASSUM ``!n'. _`` [`n'`] >>
+REV_FULL_SIMP_TAC std_ss []
+);
+
+val weak_invar_conj1_thm = prove(``
+  !m.
+  weak_model m ==>
+  !ms invar1 invar2 ls ms'.
+  (m.weak ms (\ms. (invar1 ms) /\ (invar2 ms)) ls ms') ==>
+  (m.weak ms invar1 ls ms') /\ (m.weak ms invar2 ls ms')``,
+
+REPEAT STRIP_TAC >> (
+  REV_FULL_SIMP_TAC std_ss [weak_model_def] >>
+  Q.EXISTS_TAC `n` >>
+  FULL_SIMP_TAC std_ss [] >>
+  REPEAT STRIP_TAC >>
+  QSPECL_X_ASSUM ``!n'. _`` [`n'`] >>
+  REV_FULL_SIMP_TAC std_ss []
+)
+);
+
+val weak_invar_conj2_thm = prove(``
+  !m.
+  weak_model m ==>
+  !ms invar1 invar2 ls ms'.
+  (m.weak ms invar1 ls ms') ==>
+  (m.weak ms invar2 ls ms') ==>
+  (m.weak ms (\ms. (invar1 ms) /\ (invar2 ms)) ls ms')``,
+
+REPEAT STRIP_TAC >>
+REV_FULL_SIMP_TAC std_ss [weak_model_def] >>
+Q.EXISTS_TAC `MIN n n'` >>
+Cases_on `n < n'` >> (
+  FULL_SIMP_TAC std_ss [arithmeticTheory.MIN_DEF] >>
+  REPEAT STRIP_TAC >>
+  QSPECL_X_ASSUM ``!n'. _`` [`n''`] >>
+  QSPECL_X_ASSUM ``!n''. _`` [`n''`] >>
+  REV_FULL_SIMP_TAC std_ss [] >>
+  FULL_SIMP_TAC std_ss []
+)
+);
+
 
 (* Definition of the triple *)
 (* Pre and post usually have conditions on execution mode and code in memory *)
 (* also post is usually a map that depends on the end state address *)
 val weak_triple_def = Define `
-  weak_triple m (l:'a) (ls:'a->bool) pre post =
+  weak_triple m (l:'b) (invar:'a->bool) (ls:'b->bool) pre post =
   !ms .
    ((m.pc ms) = l) ==> (pre ms) ==>
-   ?ms'. ((m.weak ms ls ms') /\
+   ?ms'. ((m.weak ms invar ls ms') /\
     (post ms'))
 `;
 
 
 val weak_case_rule_thm = prove(``
-!m l ls pre post C1.
-  weak_triple m l ls (\ms. (pre ms) /\ (C1 ms)) post ==>
-  weak_triple m l ls (\ms. (pre ms) /\ (~(C1 ms))) post ==>
-  weak_triple m l ls pre post
+!m l invar1 invar2 ls pre post C1.
+  weak_model m ==>
+  weak_triple m l invar1 ls (\ms. (pre ms) /\ (C1 ms)) post ==>
+  weak_triple m l invar2 ls (\ms. (pre ms) /\ (~(C1 ms))) post ==>
+  weak_triple m l (\ms. (invar1 ms) \/ (invar2 ms)) ls pre post
 ``,
 
-REPEAT STRIP_TAC >>
 FULL_SIMP_TAC std_ss [weak_triple_def] >>
-METIS_TAC []
+REPEAT STRIP_TAC >>
+Cases_on `C1 ms` >> (
+  RES_TAC >>
+  Q.EXISTS_TAC `ms'` >>
+  FULL_SIMP_TAC std_ss [weak_model_def]
+(* Manually specialising the first assumption speeds up the proof significantly... *)
+) >| [
+  QSPECL_X_ASSUM ``!ms invar ls ms'. _`` [`ms:'a`, `invar1:'a -> bool`, `ls:'b -> bool`, `ms':'a`] >>
+  METIS_TAC [],
+
+  QSPECL_X_ASSUM ``!ms invar ls ms'. _`` [`ms:'a`, `invar2:'a -> bool`, `ls:'b -> bool`, `ms':'a`] >>
+  METIS_TAC []
+]
 );
+
 
 val weak_weakening_rule_thm =
   store_thm("weak_weakening_rule_thm",
   ``!m. 
-    !l ls pre1 pre2 post1 post2.
+    !l invar1 invar2 ls pre1 pre2 post1 post2.
     weak_model m ==>
     (!ms. ((m.pc ms) = l) ==> (pre2 ms) ==> (pre1 ms)) ==>
     (!ms. ((m.pc ms) IN ls) ==> (post1 ms) ==> (post2 ms)) ==>
-    weak_triple m l ls pre1 post1 ==>
-    weak_triple m l ls pre2 post2
+    (* You could maybe prove a stronger theorem where this antecedent
+     * has to be true only for the states along the execution... *)
+    (!ms. ((invar1 ms) ==> (invar2 ms))) ==>
+    weak_triple m l invar1 ls pre1 post1 ==>
+    weak_triple m l invar2 ls pre2 post2
   ``,
 
 SIMP_TAC std_ss [weak_triple_def] >>
 REPEAT STRIP_TAC >>
-METIS_TAC [weak_pc_in_thm]
+IMP_RES_TAC weak_pc_in_thm >>
+subgoal `?ms'. m.weak ms invar1 ls ms' /\ post1 ms'` >- (
+  RES_TAC >>
+  METIS_TAC []
+) >>
+Q.EXISTS_TAC `ms'` >>
+subgoal `post2 ms'` >- (
+   METIS_TAC []
+) >>
+METIS_TAC [weak_invar_weak_thm]
 );
-
 
 
 val weak_subset_rule_thm =
  store_thm("weak_subset_rule_thm",
-  ``!m.  ! l ls1 ls2 pre post .
+  ``!m l invar ls1 ls2 pre post .
     weak_model m ==>
     (!ms. ((post ms) ==> (~((m.pc ms) IN ls2)))) ==>
-    weak_triple m l (ls1 UNION ls2) pre post ==>
-    weak_triple m l ls1 pre post``,
+    weak_triple m l invar (ls1 UNION ls2) pre post ==>
+    weak_triple m l invar ls1 pre post``,
 
 REPEAT STRIP_TAC >>
 REV_FULL_SIMP_TAC std_ss [weak_triple_def] >>
@@ -218,21 +298,20 @@ METIS_TAC [weak_union_pc_not_in_thm]
 );
 
 
-
 val weak_seq_rule_thm = store_thm("weak_seq_rule_thm",
-  ``!m l ls1 ls2 pre post.
+  ``!m l invar ls1 ls2 pre post.
     weak_model m ==>
-    weak_triple m l (ls1 UNION ls2) pre post ==>
+    weak_triple m l invar (ls1 UNION ls2) pre post ==>
     (!l1. (l1 IN ls1) ==>
-    (weak_triple m l1 ls2 post post)) ==>
-    weak_triple m l ls2 pre post``,
+    (weak_triple m l1 invar ls2 post post)) ==>
+    weak_triple m l invar ls2 pre post``,
 
 REPEAT STRIP_TAC >>
 SIMP_TAC std_ss [weak_triple_def] >>
 REPEAT STRIP_TAC >>
-PAT_X_ASSUM ``(weak_triple m l (ls1 UNION ls2) pre  post)``
+PAT_X_ASSUM ``(weak_triple m l invar (ls1 UNION ls2) pre post)``
               (fn thm => ASSUME_TAC (SIMP_RULE std_ss [weak_triple_def] thm)) >>
-QSPECL_X_ASSUM ``!x.P`` [`ms`] >>
+QSPECL_X_ASSUM ``!ms. _`` [`ms`] >>
 REV_FULL_SIMP_TAC std_ss [] >>
 Cases_on `(m.pc ms') IN ls2` >- (
   METIS_TAC [weak_union2_thm]
@@ -240,46 +319,49 @@ Cases_on `(m.pc ms') IN ls2` >- (
 Q.SUBGOAL_THEN `(m.pc ms') IN ls1` ASSUME_TAC >- (
   METIS_TAC [weak_union_thm, weak_pc_in_thm]
 ) >>
-QSPECL_X_ASSUM  ``!l1. _`` [`m.pc ms'`] >>
+QSPECL_X_ASSUM  ``!l1. _`` [`m.pc (ms':'a)`] >>
 REV_FULL_SIMP_TAC std_ss [weak_triple_def] >>
 QSPECL_X_ASSUM  ``!m. _`` [`ms'`] >>
-REV_FULL_SIMP_TAC std_ss[] >>
+REV_FULL_SIMP_TAC std_ss [] >>
 ASSUME_TAC (Q.SPECL [`m`] weak_comp_thm) >>
 METIS_TAC []
 );
 
+
 val weak_conj_rule_thm = prove(``
   !m.
   weak_model m ==>
-  !l ls pre post1 post2.
-  weak_triple m l ls pre post1 ==>
-  weak_triple m l ls pre post2 ==>
-  weak_triple m l ls pre (\ms. (post1 ms) /\ (post2 ms))``,
+  !l invar1 invar2 ls pre post1 post2.
+  weak_triple m l invar1 ls pre post1 ==>
+  weak_triple m l invar2 ls pre post2 ==>
+  weak_triple m l (\ms. (invar1 ms) /\ (invar2 ms)) ls pre (\ms. (post1 ms) /\ (post2 ms))``,
 
 REPEAT STRIP_TAC >>
 FULL_SIMP_TAC std_ss [weak_triple_def] >>
 REPEAT STRIP_TAC >>
-METIS_TAC [weak_unique_thm]
+subgoal `?ms'. post1 ms' /\ post2 ms'` >- (
+  METIS_TAC [weak_unique_thm]
+) >>
+METIS_TAC [weak_unique_thm, weak_invar_conj2_thm]
 );
 
 
-
 val weak_loop_step_def = Define `
- weak_loop_step m ms var l le invariant C1 =
- let x:num = var ms in
- (\ms'. (m.weak ms ({l} UNION le) ms') /\
-       ((invariant ms) /\ (C1 ms)) /\
-       (((m.pc ms')=l) /\ (invariant ms') /\ ((var ms') < x) /\ ((var ms') >= 0))
-       )
-       `;
+  weak_loop_step m ms var l invar le loop_invar C1 =
+    let x:num = var ms in
+      (\ms'. (m.weak ms invar ({l} UNION le) ms') /\
+        ((loop_invar ms) /\ (C1 ms)) /\
+        (((m.pc ms') = l) /\ (loop_invar ms') /\ ((var ms') < x) /\ ((var ms') >= 0))
+      )
+`;
 
-val loop_fun_defn =
-       Hol_defn "loop_fun" `
-loop_fun m ms var l le invariant C1  =
-let MS' = weak_loop_step m ms var l le invariant C1 in
-if MS' = {} then ms
-else let ms' = (CHOICE MS') in
-  (loop_fun m ms' var l le invariant C1)
+val loop_fun_defn = Hol_defn "loop_fun" `
+  loop_fun m ms var l invar le loop_invar C1  =
+    let MS' = weak_loop_step m ms var l invar le loop_invar C1 in
+      if MS' = {}
+      then ms
+      else let ms' = (CHOICE MS') in
+             (loop_fun m ms' var l invar le loop_invar C1)
 `;
 
 (*
@@ -287,12 +369,12 @@ Defn.tgoal loop_fun_defn
 *)
 val (loop_fun_eqns, loop_fun_ind) = Defn.tprove(loop_fun_defn,
   FULL_SIMP_TAC std_ss [weak_loop_step_def] >>
-  WF_REL_TAC `measure (\(m, ms,var,l,le,invariant,C1). var ms)` >>
+  WF_REL_TAC `measure (\(m, ms, var, l, invar, le, loop_invar, C1). var ms)` >>
   REPEAT STRIP_TAC >>
   REV_FULL_SIMP_TAC std_ss [LET_DEF] >>
   Q.ABBREV_TAC `MS' =  (\ms'.
-               m.weak ms ({l} UNION le) ms' /\ (invariant ms /\ C1 ms) /\
-               ((m.pc ms') = l) /\ invariant ms' /\ var ms' < var ms)` >>
+               m.weak ms invar ({l} UNION le) ms' /\ (loop_invar ms /\ C1 ms) /\
+               ((m.pc ms') = l) /\ loop_invar ms' /\ var ms' < var ms)` >>
   ASSUME_TAC (ISPEC ``MS':'a->bool`` pred_setTheory.CHOICE_DEF)  >>
   REV_FULL_SIMP_TAC std_ss [] >>
   FULL_SIMP_TAC std_ss [Abbr `MS'`, pred_setTheory.IN_ABS]
@@ -300,121 +382,106 @@ val (loop_fun_eqns, loop_fun_ind) = Defn.tprove(loop_fun_defn,
 
 
 val weak_loop_contract_def = Define `
-  weak_loop_contract m l le invariant C1 var =
+  weak_loop_contract m l invar le loop_invar C1 var =
     (~(l IN le)) /\
-    (!x. (weak_triple m l ({l} UNION le) (\ms. (invariant ms) /\ (C1 ms) /\ ((var ms) = x:num))
-         (\ms.(((m.pc ms)=l) /\ (invariant ms) /\ ((var ms) < x) /\ ((var ms) >= 0)))))
+    (!x. (weak_triple m l invar ({l} UNION le) (\ms. (loop_invar ms) /\ (C1 ms) /\ ((var ms) = x:num))
+         (\ms.(((m.pc ms) = l) /\ (loop_invar ms) /\ ((var ms) < x) /\ ((var ms) >= 0)))))
 `;
 
-val inductive_invariant_goal = (fst o dest_imp o concl ) (
-Q.SPEC `(\m ms var l le invariant C1.
-weak_model m ==>
-weak_loop_contract m l le invariant C1 var ==>
-weak_triple m l le (\ms. (invariant ms) /\ (~(C1 ms))) post ==>
-((invariant ms) /\ ((m.pc ms) = l) /\ (C1 ms)) ==>
- (?ms'. ((m.weak ms le ms') /\ (post ms'))))` loop_fun_ind);
+val inductive_loop_invar_goal = (fst o dest_imp o concl) (
+  Q.SPEC `(\m ms var l invar le loop_invar C1.
+           weak_model m ==>
+           weak_loop_contract m l invar le loop_invar C1 var ==>
+           weak_triple m l invar le (\ms. (loop_invar ms) /\ (~(C1 ms))) post ==>
+           ((loop_invar ms) /\ ((m.pc ms) = l) /\ (C1 ms)) ==>
+           (?ms'. ((m.weak ms invar le ms') /\ (post ms')))
+          )`
+         loop_fun_ind
+);
 
-
-val inductive_invariant_thm = prove(``
-^inductive_invariant_goal
+val inductive_loop_invar_thm = prove(``
+^inductive_loop_invar_goal
 ``,
 
 REPEAT STRIP_TAC >>
 FULL_SIMP_TAC std_ss [] >>
 REPEAT STRIP_TAC >>
-(* We first prove that one iteration works *)
-SUBGOAL_THEN ``(weak_loop_step m ms var l le invariant C1) <> {}`` ASSUME_TAC  >- (
-  SIMP_TAC std_ss [weak_loop_step_def, LET_DEF] >>
+(* We first prove that one iteration works, i.e. that there is an ending state for
+ * the weak transition. *)
+subgoal `(weak_loop_step m ms var l invar le loop_invar C1) <> {}` >- (
+  SIMP_TAC std_ss [weak_loop_step_def, LET_DEF, GSYM pred_setTheory.MEMBER_NOT_EMPTY] >>
   FULL_SIMP_TAC std_ss [weak_loop_contract_def] >>
   QSPECL_X_ASSUM ``!x. _`` [`(var (ms)):num`] >>
   FULL_SIMP_TAC std_ss [weak_triple_def] >>
-  QSPECL_X_ASSUM ``!x. _`` [`ms`] >>
+  QSPECL_X_ASSUM ``!ms'. _`` [`ms`] >>
   REV_FULL_SIMP_TAC std_ss [] >>
-  FULL_SIMP_TAC std_ss [GSYM pred_setTheory.MEMBER_NOT_EMPTY] >>
   EXISTS_TAC ``ms'':'a`` >>
   FULL_SIMP_TAC std_ss [pred_setTheory.SPECIFICATION]
 ) >>
 FULL_SIMP_TAC std_ss [] >>
 
-Q.ABBREV_TAC `MS' = (weak_loop_step m ms var l le invariant C1)` >>
+Q.ABBREV_TAC `MS' = (weak_loop_step m ms var l invar le loop_invar C1)` >>
 Q.ABBREV_TAC `ms' = CHOICE MS'` >>
 
-(* We prove that the invariant is preserved *)
-SUBGOAL_THEN ``(weak_loop_step m ms var l le invariant C1) ms'`` ASSUME_TAC >- (
+(* We prove that the loop invariant is preserved in ms' *)
+subgoal `(weak_loop_step m ms var l invar le loop_invar C1) ms'` >- (
   FULL_SIMP_TAC std_ss [Abbr `ms'`] >>
   ASSUME_TAC (ISPEC ``MS':'a->bool`` pred_setTheory.CHOICE_DEF) >>
   REV_FULL_SIMP_TAC std_ss [pred_setTheory.SPECIFICATION]
 ) >>
-Q.SUBGOAL_THEN `invariant ms'` ASSUME_TAC >- (
-  FULL_SIMP_TAC std_ss [ weak_loop_step_def, LET_DEF]
+subgoal `loop_invar ms'` >- (
+  FULL_SIMP_TAC std_ss [weak_loop_step_def, LET_DEF]
 ) >>
 FULL_SIMP_TAC std_ss [] >>
-Q.SUBGOAL_THEN `(m.pc ms') = l` ASSUME_TAC >- (
-  FULL_SIMP_TAC std_ss [ weak_loop_step_def, LET_DEF]
+subgoal `(m.pc ms') = l` >- (
+  FULL_SIMP_TAC std_ss [weak_loop_step_def, LET_DEF]
 ) >>
 FULL_SIMP_TAC std_ss [] >>
 
 (* If we exit the loop *)
-Cases_on `~ (C1 ms')` >- (
-  (FULL_SIMP_TAC std_ss [weak_loop_step_def, LET_DEF]) >>
-  (FULL_SIMP_TAC std_ss [weak_triple_def]) >>
-  QSPECL_X_ASSUM  ``!x. _`` [`ms'`] >>
-  (REV_FULL_SIMP_TAC std_ss []) >>
-  ASSUME_TAC (Q.SPECL [`m`] weak_comp_thm) >>
-  REV_FULL_SIMP_TAC std_ss [] >>
-  QSPECL_X_ASSUM ``!x. _`` [`ms`, `{l}`, `le`, `ms'`, `ms''`] >>
-  REV_FULL_SIMP_TAC (std_ss) [SINGLETONS_UNION_thm] >>
-  Q.SUBGOAL_THEN `l NOTIN le` (FULLSIMP_BY_THM std_ss) >- (
-    FULL_SIMP_TAC std_ss [weak_loop_contract_def, pred_setTheory.IN_SING]
-  ) >>
-  METIS_TAC []
-) >> (
-  FULL_SIMP_TAC std_ss []
-) >> (
+Cases_on `~(C1 ms')` >> (
   FULL_SIMP_TAC std_ss [weak_loop_step_def, LET_DEF]
-) >>
-ASSUME_TAC (Q.SPECL [`m`] weak_comp_thm) >>
-REV_FULL_SIMP_TAC std_ss [] >>
-QSPECL_X_ASSUM ``!x. _`` [`ms`, `{l}`, `le`, `ms'`, `ms''`] >>
-REV_FULL_SIMP_TAC (std_ss) [SINGLETONS_UNION_thm] >>
-  Q.SUBGOAL_THEN `l NOTIN le` (FULLSIMP_BY_THM std_ss) >- (
-    FULL_SIMP_TAC std_ss [weak_loop_contract_def, pred_setTheory.IN_SING]
-  ) >>
-  METIS_TAC []
+) THEN_LT TACS_TO_LT [ 
+  FULL_SIMP_TAC std_ss [weak_triple_def],
+
+  ALL_TAC
+] >> (
+  METIS_TAC [weak_comp_thm, weak_loop_contract_def, pred_setTheory.IN_SING]
+)
 );
 
 
+val loop_invar_rule_tmp_thm = 
+  MP 
+    (Q.SPEC `(\m ms var l invar le loop_invar C1.
+	     weak_model m ==>
+	     weak_loop_contract m l invar le loop_invar C1 var ==>
+	     weak_triple m l invar le (\ms. (loop_invar ms) /\ (~(C1 ms))) post ==>
+	     ((loop_invar ms) /\ ((m.pc ms) = l) /\ (C1 ms)) ==>
+	     (?ms'. ((m.weak ms invar le ms') /\ (post ms'))))`
+	     loop_fun_ind
+    )
+    inductive_loop_invar_thm;
 
-
-val invariant_rule_tmp_thm = 
-MP 
-(Q.SPEC `(\m ms var l le invariant C1.
-weak_model m ==>
-weak_loop_contract m l le invariant C1 var ==>
-weak_triple m l le (\ms. (invariant ms) /\ (~(C1 ms))) post ==>
-((invariant ms) /\ ((m.pc ms) = l) /\ (C1 ms)) ==>
- (?ms'. ((m.weak ms le ms') /\ (post ms'))))` loop_fun_ind) inductive_invariant_thm;
-
-val weak_invariant_rule_thm = store_thm("weak_invariant_rule_thm",
+val weak_loop_invar_rule_thm = store_thm("weak_loop_invar_rule_thm",
   ``!m.
     weak_model m ==>
-    !l le invariant C1 var post.
-    weak_loop_contract m l le invariant C1 var ==>
-    weak_triple m l le (\ms. (invariant ms) /\ (~(C1 ms))) post ==>
-    weak_triple m l le invariant post``,
+    !l invar le loop_invar C1 var post.
+    weak_loop_contract m l invar le loop_invar C1 var ==>
+    weak_triple m l invar le (\ms. (loop_invar ms) /\ (~(C1 ms))) post ==>
+    weak_triple m l invar le loop_invar post``,
 
 REPEAT STRIP_TAC >>
 SIMP_TAC std_ss [weak_triple_def] >>
 REPEAT STRIP_TAC >>
-ASSUME_TAC (Q.SPECL [`m`, `ms`, `var`, `l`, `le`, `invariant`, `C1`] invariant_rule_tmp_thm) >>
-FULL_SIMP_TAC std_ss [] >>
+ASSUME_TAC (Q.SPECL [`m`, `ms`, `var`, `l`, `invar`, `le`, `loop_invar`, `C1`]
+                    loop_invar_rule_tmp_thm
+           ) >>
 REV_FULL_SIMP_TAC std_ss [] >>
 Cases_on `C1 ms` >- (
-  FULL_SIMP_TAC std_ss [] >>
-  Q.EXISTS_TAC `ms'`>>
-  FULL_SIMP_TAC std_ss []
+  METIS_TAC []
 ) >>
-FULL_SIMP_TAC std_ss [weak_triple_def] 
+FULL_SIMP_TAC std_ss [weak_triple_def]
 );
 
 val _ = export_theory();
