src/theory/bin_hoare_logic/bin_simp_hoare_logicScript.sml
@@ -9,33 +9,38 @@ val _ = new_theory "bin_simp_hoare_logic";
 (* Inv is usually the fact that the program is in memory and that
  * the execution mode is the expected one *)
 val weak_map_triple_def = Define `
-  weak_map_triple m invariant (l:'a) (ls:'a->bool) (ls':'a->bool) pre post =
+  weak_map_triple (m:('a, 'b) bin_model_t) invar l ls ls' pre post =
     (((ls INTER ls') = EMPTY) /\
-     (weak_triple m l (ls UNION ls')
-                 (\ms. (pre ms) /\ (invariant ms))
-                 (\ms. if ((m.pc ms) IN ls') then F else ((post ms) /\ (invariant ms)))
+     (weak_triple m l invar (ls UNION ls')
+                 (\ms. pre ms)
+                 (\ms. if ((m.pc ms) IN ls') then F else (post ms))
      )
     )
 `;
 
+
 val weak_map_subset_blacklist_rule_thm = prove(``
-  !m.
-  !invariant. !l ls ls' ls'' pre post.
+  !m invar l ls ls' ls'' pre post.
   weak_model m ==>
   ls'' SUBSET ls' ==>
-  weak_map_triple m invariant l ls ls' pre post ==>
-  weak_map_triple m invariant l ls ls'' pre post``,
+  weak_map_triple m invar l ls ls' pre post ==>
+  weak_map_triple m invar l ls ls'' pre post``,
 
 REPEAT STRIP_TAC >>
 FULL_SIMP_TAC std_ss [weak_map_triple_def] >>
 ASSUME_TAC (ISPECL [``ls'':'b->bool``, ``ls':'b->bool``, ``ls:'b->bool``] INTER_SUBSET_EMPTY_thm) >>
 REV_FULL_SIMP_TAC std_ss [] >>
-ASSUME_TAC (ISPECL [``ls'':'b->bool``, ``ls':'b->bool``] SUBSET_EQ_UNION_thm) >>
+irule weak_weakening_rule_thm >>
+subgoal `?v. ls' = ls'' UNION v` >- (
+  METIS_TAC [SUBSET_EQ_UNION_thm]
+) >>
 REV_FULL_SIMP_TAC std_ss [] >>
 FULL_SIMP_TAC std_ss [] >>
-Q.SUBGOAL_THEN `!ms.
-                ((\ms. m.pc ms NOTIN ls'' UNION v /\ post ms /\ invariant ms)) ms ==>
-                m.pc ms NOTIN v` ASSUME_TAC >- (
+Q.EXISTS_TAC `invar` >>
+Q.EXISTS_TAC `(\ms:'a. m.pc ms NOTIN (ls'':'b->bool) UNION v /\ post ms)` >>
+Q.EXISTS_TAC `\ms. pre ms` >>
+subgoal `!ms. ((\ms. m.pc ms NOTIN ls'' UNION v /\ post ms)) ms ==>
+              m.pc ms NOTIN v` >- (
   REPEAT STRIP_TAC >>
   FULL_SIMP_TAC (std_ss++pred_setSimps.PRED_SET_AC_ss++pred_setSimps.PRED_SET_ss) [] 
 ) >>
@@ -43,34 +48,28 @@ Q.SUBGOAL_THEN `(ls UNION (ls'' UNION v)) = ((ls UNION ls'') UNION v)`
   (fn thm => FULL_SIMP_TAC std_ss [thm]) >- (
   FULL_SIMP_TAC (std_ss++pred_setSimps.PRED_SET_AC_ss++pred_setSimps.PRED_SET_ss) []
 ) >>
-ASSUME_TAC (Q.SPECL [`m`, `l`, `ls UNION ls''`, `v`,
-	   `\ms:'a. pre ms /\ invariant ms`,
-	   `\ms:'a. m.pc ms NOTIN (ls'':'b->bool) UNION v /\ post ms /\ invariant ms`] 
+ASSUME_TAC (Q.SPECL [`m`, `l`, `invar`, `ls UNION ls''`, `v`,
+	   `\ms:'a. pre ms`,
+	   `\ms:'a. m.pc ms NOTIN (ls'':'b->bool) UNION v /\ post ms`] 
   weak_subset_rule_thm) >>
 REV_FULL_SIMP_TAC std_ss [] >>
-Q.SUBGOAL_THEN `!ms. ((m.pc ms) IN (ls UNION ls'')) ==>
-                ((\ms. m.pc ms NOTIN ls'' UNION v /\ post ms /\ invariant ms) ms) ==>
-                ((\ms. m.pc ms NOTIN ls'' /\ post ms /\ invariant ms) ms)` ASSUME_TAC >- (
+subgoal `!ms. ((m.pc ms) IN (ls UNION ls'')) ==>
+              ((\ms. m.pc ms NOTIN ls'' UNION v /\ post ms) ms) ==>
+              ((\ms. m.pc ms NOTIN ls'' /\ post ms) ms)` >- (
   REPEAT STRIP_TAC >>
   FULL_SIMP_TAC (std_ss++pred_setSimps.PRED_SET_AC_ss++pred_setSimps.PRED_SET_ss) []
 ) >>
-ASSUME_TAC (Q.SPECL [`m`, `l`, `ls UNION ls''`,
-           `(\ms. pre ms /\ invariant ms)`, `(\ms. pre ms /\ invariant ms)`,
-           `(\ms:'a. m.pc ms NOTIN (ls'':'b->bool) UNION v /\ post ms /\ invariant ms)`,
-           `(\ms:'a. m.pc ms NOTIN (ls'':'b->bool) /\ post ms /\ invariant ms)`
-           ] 
-  weak_weakening_rule_thm) >>
-REV_FULL_SIMP_TAC std_ss []
+METIS_TAC []
 );
 
 
 val weak_map_move_to_blacklist = store_thm("weak_map_move_to_blacklist",
-  ``!m invariant l l' ls ls' ls'' pre post.
+  ``!m invar l l' ls ls' pre post.
     weak_model m ==>
     l' IN ls ==>
     (!ms. (m.pc ms = l') ==> (post ms = F)) ==>
-    weak_map_triple m invariant l ls ls' pre post ==>
-    weak_map_triple m invariant l (ls DELETE l') (l' INSERT ls') pre post``,
+    weak_map_triple m invar l ls ls' pre post ==>
+    weak_map_triple m invar l (ls DELETE l') (l' INSERT ls') pre post``,
 
 REPEAT STRIP_TAC >>
 FULL_SIMP_TAC std_ss [weak_map_triple_def, weak_triple_def] >>
@@ -109,160 +108,163 @@ REPEAT STRIP_TAC >| [
 ]
 );
 
+
 val weak_map_weakening_rule_thm = store_thm("weak_map_weakening_rule_thm",
-  ``!m invariant l ls ls' pre post1 post2.
+  ``!m invar l ls ls' pre post1 post2.
     weak_model m ==>
     (!ms. (m.pc ms) IN ls ==> (post1 ms) ==> (post2 ms)) ==>
-    weak_map_triple m invariant l ls ls' pre post1 ==>
-    weak_map_triple m invariant l ls ls' pre post2``,
+    weak_map_triple m invar l ls ls' pre post1 ==>
+    weak_map_triple m invar l ls ls' pre post2``,
 
 REPEAT STRIP_TAC >>
 FULL_SIMP_TAC std_ss [weak_map_triple_def] >>
+irule weak_weakening_rule_thm >>
+FULL_SIMP_TAC std_ss [] >>
+Q.EXISTS_TAC `invar` >>
+Q.EXISTS_TAC `\ms. m.pc ms NOTIN (ls':'b->bool) /\ post1 ms` >>
+Q.EXISTS_TAC `\ms. pre ms` >>
 subgoal `!ms. m.pc ms IN (ls UNION ls') ==>
-         (\ms. m.pc ms NOTIN ls' /\ post1 ms /\ invariant ms) ms ==>
-         (\ms. m.pc ms NOTIN ls' /\ post2 ms /\ invariant ms) ms` >- (
+         (\ms. m.pc ms NOTIN ls' /\ post1 ms) ms ==>
+         (\ms. m.pc ms NOTIN ls' /\ post2 ms) ms` >- (
   REPEAT STRIP_TAC >>
   FULL_SIMP_TAC (std_ss++pred_setSimps.PRED_SET_AC_ss++pred_setSimps.PRED_SET_ss) []
 ) >>
-ASSUME_TAC (Q.SPECL [`m`, `l`, `ls UNION ls'`, `\ms. pre ms /\ invariant ms`, 
-                     `\ms. pre ms /\ invariant ms`,
-                     `\ms. m.pc ms NOTIN (ls':'b->bool) /\ post1 ms /\ invariant ms`,
-                     `\ms. m.pc ms NOTIN (ls':'b->bool) /\ post2 ms /\ invariant ms`]
-  weak_weakening_rule_thm) >>
 REV_FULL_SIMP_TAC std_ss []
 );
 
 val weak_map_strengthening_rule_thm = store_thm("weak_map_strengthening_rule_thm",
-  ``!m invariant l ls ls' pre1 pre2 post.
+  ``!m invar l ls ls' pre1 pre2 post.
     weak_model m ==>
     (!ms. ((m.pc ms) = l) ==> (pre2 ms) ==> (pre1 ms)) ==>
-    weak_map_triple m invariant l ls ls' pre1 post ==>
-    weak_map_triple m invariant l ls ls' pre2 post``,
+    weak_map_triple m invar l ls ls' pre1 post ==>
+    weak_map_triple m invar l ls ls' pre2 post``,
 
 REPEAT STRIP_TAC >>
 FULL_SIMP_TAC std_ss [weak_map_triple_def] >>
+irule weak_weakening_rule_thm >>
+FULL_SIMP_TAC std_ss [] >>
+Q.EXISTS_TAC `invar` >>
+Q.EXISTS_TAC `\ms. m.pc ms NOTIN (ls':'b->bool) /\ post ms` >>
+Q.EXISTS_TAC `\ms. pre1 ms` >>
 subgoal `!ms. (m.pc ms = l) ==>
-         (\ms. pre2 ms /\ invariant ms) ms ==>
-         (\ms. pre1 ms /\ invariant ms) ms` >- (
+         (\ms. pre2 ms) ms ==>
+         (\ms. pre1 ms) ms` >- (
   REPEAT STRIP_TAC >>
   FULL_SIMP_TAC (std_ss++pred_setSimps.PRED_SET_AC_ss++pred_setSimps.PRED_SET_ss) []
 ) >>
-ASSUME_TAC (Q.SPECL [`m`, `l`, `ls UNION ls'`, `\ms. pre1 ms /\ invariant ms`, 
-                     `\ms. pre2 ms /\ invariant ms`,
-                     `\ms. m.pc ms NOTIN (ls':'b->bool) /\ post ms /\ invariant ms`,
-                     `\ms. m.pc ms NOTIN (ls':'b->bool) /\ post ms /\ invariant ms`]
-  weak_weakening_rule_thm) >>
 REV_FULL_SIMP_TAC std_ss []
 );
 
 
 val weak_map_add_post_corollary_thm = prove(``
-  !m invariant l ls ls' pre post1 post2.
+  !m invar l ls ls' pre post1 post2.
   weak_model m ==>
-  weak_map_triple m invariant l ls ls' pre post1 ==>
-  weak_map_triple m invariant l ls ls' pre (\ms. if m.pc ms IN ls then post1 ms else post2 ms)``,
+  weak_map_triple m invar l ls ls' pre post1 ==>
+  weak_map_triple m invar l ls ls' pre (\ms. if m.pc ms IN ls then post1 ms else post2 ms)``,
 
 REPEAT STRIP_TAC >>
-ASSUME_TAC (Q.SPECL [`m`, `invariant`, `l`, `ls`, `ls'`, `pre`,  `post1`, 
-                     `(\ms. if m.pc ms IN ls then post1 ms else post2 ms)`]
-  weak_map_weakening_rule_thm) >>
+irule weak_map_weakening_rule_thm >>
+FULL_SIMP_TAC std_ss [] >>
+Q.EXISTS_TAC `post1` >>
 REV_FULL_SIMP_TAC std_ss []
 );
 
 
 val weak_map_add_post2_corollary = prove(``
-  !m invariant l ls1 ls2 ls' pre post1 post2.
+  !m invar l ls1 ls2 ls' pre post1 post2.
   weak_model m ==>
   ((ls1 INTER ls2) = EMPTY) ==>
-  weak_map_triple m invariant l ls1 ls' pre post1 ==>
-  weak_map_triple m invariant l ls1 ls' pre (\ms. if (m.pc ms IN ls2) then post2 ms else post1 ms)``,
+  weak_map_triple m invar l ls1 ls' pre post1 ==>
+  weak_map_triple m invar l ls1 ls' pre (\ms. if (m.pc ms IN ls2) then post2 ms else post1 ms)``,
 
 REPEAT STRIP_TAC >>
+irule weak_map_weakening_rule_thm >>
+FULL_SIMP_TAC std_ss [] >>
+Q.EXISTS_TAC `post1` >>
 subgoal `!ms. m.pc ms IN ls1 ==> post1 ms ==>
          (\ms. if m.pc ms IN ls2 then post2 ms else post1 ms) ms` >- (
   REPEAT STRIP_TAC >>
   METIS_TAC [INTER_EMPTY_IN_NOT_IN_thm]
 ) >>
-ASSUME_TAC (Q.SPECL [`m`, `invariant`, `l`, `ls1`, `ls'`, `pre`,  `post1`,
-                     `\ms. if m.pc ms IN ls2 then post2 ms else post1 ms`]
-  weak_map_weakening_rule_thm) >>
 REV_FULL_SIMP_TAC std_ss [] 
 );
 
 
 (* This proof should use the blacklist move lemma *)
 val weak_map_seq_thm = prove(
-  ``!m invariant l ls1 ls ls' pre post.
+  ``!m invar l ls1 ls ls' pre post.
     weak_model m ==>
     (ls INTER ls' = {}) ==>
-    weak_map_triple m invariant l ls1 (ls UNION ls') pre post ==>
+    weak_map_triple m invar l ls1 (ls UNION ls') pre post ==>
     (!l1.
      (l1 IN ls1) ==>
-     weak_map_triple m invariant l1 ls ls' post post
+     weak_map_triple m invar l1 ls ls' post post
     ) ==>
-    (weak_map_triple m invariant l ls ls' pre post)``,
+    (weak_map_triple m invar l ls ls' pre post)``,
 
 REPEAT STRIP_TAC >>
 FULL_SIMP_TAC std_ss [weak_map_triple_def] >>
-REV_FULL_SIMP_TAC std_ss [] >>
+irule weak_seq_rule_thm >>
+FULL_SIMP_TAC std_ss [] >>
+Q.EXISTS_TAC `ls1` >>
 (* Massage first contract *)
-subgoal `(!ms. m.pc ms IN (ls1 UNION (ls UNION ls')) ==>
-         (\ms. m.pc ms NOTIN ls UNION ls' /\ post ms /\ invariant ms) ms ==>
-         (\ms. m.pc ms NOTIN ls' /\ post ms /\ invariant ms) ms)` >- (
-  FULL_SIMP_TAC (std_ss++pred_setSimps.PRED_SET_AC_ss++pred_setSimps.PRED_SET_ss) []
+subgoal `weak_triple m l invar (ls1 UNION (ls UNION ls')) (\ms. pre ms)
+           (\ms. m.pc ms NOTIN ls' /\ post ms)` >- (
+  irule weak_weakening_rule_thm >>
+  FULL_SIMP_TAC std_ss [] >>
+  Q.EXISTS_TAC `invar` >>
+  Q.EXISTS_TAC `\ms. m.pc ms NOTIN ls UNION ls' /\ post ms` >>
+  Q.EXISTS_TAC `\ms. pre ms` >>
+  subgoal `(!ms. m.pc ms IN (ls1 UNION (ls UNION ls')) ==>
+	   (\ms. m.pc ms NOTIN ls UNION ls' /\ post ms) ms ==>
+	   (\ms. m.pc ms NOTIN ls' /\ post ms) ms)` >- (
+    FULL_SIMP_TAC (std_ss++pred_setSimps.PRED_SET_AC_ss++pred_setSimps.PRED_SET_ss) []
+  ) >>
+  FULL_SIMP_TAC std_ss []
 ) >>
-ASSUME_TAC (Q.SPECL [`m`, `l`, `ls1 UNION (ls UNION ls')`, `\ms. pre ms /\ invariant ms`,
-                     `\ms. pre ms /\ invariant ms`,
-                     `\ms. m.pc ms NOTIN ls UNION ls' /\ post ms /\ invariant ms`,
-                     `\ms. m.pc ms NOTIN ls' /\ post ms /\ invariant ms`]
-  weak_weakening_rule_thm) >>
-REV_FULL_SIMP_TAC std_ss [] >>
 (* Massage the second contract *)
 subgoal `!l1. l1 IN ls1 ==>
-         weak_triple m l1 (ls UNION ls') (\ms. m.pc ms NOTIN ls' /\ post ms /\ invariant ms)
-         (\ms. m.pc ms NOTIN ls' /\ post ms /\ invariant ms)` >- (
+         weak_triple m l1 invar (ls UNION ls') (\ms. m.pc ms NOTIN ls' /\ post ms)
+         (\ms. m.pc ms NOTIN ls' /\ post ms)` >- (
   REPEAT STRIP_TAC >>
+  irule weak_weakening_rule_thm >>
+  FULL_SIMP_TAC std_ss [] >>
+  Q.EXISTS_TAC `invar` >>
+  Q.EXISTS_TAC `\ms. m.pc ms NOTIN ls' /\ post ms` >>
+  Q.EXISTS_TAC `\ms. post ms` >>
   subgoal `!ms.
            (m.pc ms = l1) ==>
-           (\ms. post ms /\ invariant ms) ms ==>
-           (\ms. m.pc ms NOTIN ls' /\ post ms /\ invariant ms) ms` >- (
+           (\ms. post ms) ms ==>
+           (\ms. m.pc ms NOTIN ls' /\ post ms) ms` >- (
     REPEAT STRIP_TAC >>
     FULL_SIMP_TAC (std_ss++pred_setSimps.PRED_SET_AC_ss++pred_setSimps.PRED_SET_ss) [] >>
     FULL_SIMP_TAC (std_ss++pred_setSimps.PRED_SET_AC_ss++pred_setSimps.PRED_SET_ss)
       [pred_setTheory.UNION_OVER_INTER] >>
     METIS_TAC [INTER_EMPTY_IN_NOT_IN_thm]
   ) >>
-  ASSUME_TAC (Q.SPECL [`m`, `l1`, `ls UNION ls'`,
-                       `\ms. post ms /\ invariant ms`,
-                       `\ms. m.pc ms NOTIN ls' /\ post ms /\ invariant ms`,
-                       `\ms. m.pc ms NOTIN ls' /\ post ms /\ invariant ms`,
-                       `\ms. m.pc ms NOTIN ls' /\ post ms /\ invariant ms`]
-    weak_weakening_rule_thm) >>
-  REV_FULL_SIMP_TAC std_ss []
+  FULL_SIMP_TAC std_ss []
 ) >>
-
-ASSUME_TAC (Q.SPECL [`m`, `l`, `ls1`, `ls UNION ls'`,
-                     `\ms. pre ms /\ invariant ms`,
-                     `\ms. m.pc ms NOTIN ls' /\ post ms /\ invariant ms`]
-  weak_seq_rule_thm) >>
-REV_FULL_SIMP_TAC std_ss []
+FULL_SIMP_TAC std_ss []
 );
 
 
 (* We should generalize the other contract to handle set of labels *)
 val weak_map_std_seq_comp_thm = store_thm("weak_map_std_seq_comp_thm",
-  ``!m ls1 ls1' ls2 ls2' invariant l pre1 post1 post2.
+  ``!m ls1 ls1' ls2 ls2' invar l pre1 post1 post2.
     weak_model m ==>
     ls1' SUBSET ls2 ==>
     (ls1 INTER ls1' = EMPTY) ==>
     (ls1' INTER ls2' = EMPTY) ==>
-    weak_map_triple m invariant l ls1 ls2 pre1 post1 ==>
-    (!l1. (l1 IN ls1) ==> (weak_map_triple m invariant l1 ls1' ls2' post1 post2)) ==>
-    weak_map_triple m invariant l ls1' (ls2 INTER ls2') pre1 post2``,
+    weak_map_triple m invar l ls1 ls2 pre1 post1 ==>
+    (!l1. (l1 IN ls1) ==> (weak_map_triple m invar l1 ls1' ls2' post1 post2)) ==>
+    weak_map_triple m invar l ls1' (ls2 INTER ls2') pre1 post2``,
 
 REPEAT STRIP_TAC >>
+irule weak_map_weakening_rule_thm >>
+FULL_SIMP_TAC std_ss [] >>
+Q.EXISTS_TAC `(\ms. if m.pc ms IN ls1 then post1 ms else post2 ms)` >>
 (* First we extend the initial contract to have the same postcondition *)
-subgoal `weak_map_triple m invariant l ls1 ls2 pre1
+subgoal `weak_map_triple m invar l ls1 ls2 pre1
            (\ms. if m.pc ms IN ls1 then post1 ms else post2 ms)` >- (
   METIS_TAC [weak_map_add_post_corollary_thm]
 ) >>
@@ -270,34 +272,34 @@ subgoal `weak_map_triple m invariant l ls1 ls2 pre1
 subgoal `ls1' UNION (ls2 INTER ls2') SUBSET ls2` >- (
   FULL_SIMP_TAC (std_ss++pred_setSimps.PRED_SET_ss) []
 ) >>
-subgoal `weak_map_triple m invariant l ls1 (ls1' UNION ls2 INTER ls2') pre1
+subgoal `weak_map_triple m invar l ls1 (ls1' UNION ls2 INTER ls2') pre1
            (\ms. if m.pc ms IN ls1 then post1 ms else post2 ms)` >- (
   METIS_TAC [weak_map_subset_blacklist_rule_thm]
 ) >>
 (* Now, we extend the second contracts *)
 subgoal `!l1.
          l1 IN ls1 ==>
-         weak_map_triple m invariant l1 ls1' (ls2 INTER ls2')
+         weak_map_triple m invar l1 ls1' (ls2 INTER ls2')
            ((\ms. if m.pc ms IN ls1 then post1 ms else post2 ms))
              (\ms. if m.pc ms IN ls1 then post1 ms else post2 ms)` >- (
   REPEAT STRIP_TAC >>
   QSPECL_X_ASSUM ``!l1. _`` [`l1`] >>  
   REV_FULL_SIMP_TAC std_ss [] >>
   (* Now, we extend the second contract to have the same postcondition *)
-  subgoal `weak_map_triple m invariant l1 ls1' ls2' post1
+  subgoal `weak_map_triple m invar l1 ls1' ls2' post1
              (\ms. if m.pc ms IN ls1 then post1 ms else post2 ms)` >- (
     METIS_TAC [weak_map_add_post2_corollary, pred_setTheory.INTER_COMM]
   ) >>
   (* We then restrict the non-accessible addresses of the first contract *)
-  subgoal `weak_map_triple m invariant l1 ls1' (ls2 INTER ls2') post1
+  subgoal `weak_map_triple m invar l1 ls1' (ls2 INTER ls2') post1
              (\ms. if m.pc ms IN ls1 then post1 ms else post2 ms)` >- (
     METIS_TAC [weak_map_subset_blacklist_rule_thm, pred_setTheory.INTER_SUBSET]
   ) >>
   FULL_SIMP_TAC std_ss [weak_triple_def, weak_map_triple_def]
 ) >>
-subgoal `weak_map_triple m invariant l ls1' (ls2 INTER ls2') pre1
+subgoal `weak_map_triple m invar l ls1' (ls2 INTER ls2') pre1
            (\ms. if m.pc ms IN ls1 then post1 ms else post2 ms)` >- (
-  ASSUME_TAC (Q.SPECL [`m`, `invariant`, `l`, `ls1`, `ls1'`, `(ls2 INTER ls2')`,
+  ASSUME_TAC (Q.SPECL [`m`, `invar`, `l`, `ls1`, `ls1'`, `(ls2 INTER ls2')`,
                        `pre1`, `(\ms. if m.pc ms IN ls1 then post1 ms else post2 ms)`]
     weak_map_seq_thm
   ) >>
@@ -317,11 +319,7 @@ subgoal `(!ms. m.pc ms IN ls1' ==>
   FULL_SIMP_TAC std_ss [] 
 ) >>
 (* Finish everything... *)
-ASSUME_TAC (Q.SPECL [`m`, `invariant`, `l`, `ls1'`, `ls2 INTER ls2'`, `pre1`,
-                     `(\ms. if m.pc ms IN ls1 then post1 ms else post2 ms)`,
-                     `post2`]
-  weak_map_weakening_rule_thm) >>
-REV_FULL_SIMP_TAC std_ss []
+FULL_SIMP_TAC std_ss []
 );
 
 (* The below are still TODO: *)
@@ -332,9 +330,9 @@ val weak_map_std_seq_comp_thm = prove(``
 (ls1' SUBSET ls2) ==>
 (ls1 INTER ls1' = EMPTY) ==>
 (ls1' INTER ls2' = EMPTY) ==>
-(weak_map_triple m invariant l ls1 ls2 pre1 post1) ==>
-(!l1 . (l1 IN ls1) ==> (weak_map_triple m invariant l1 ls1' ls2' (post1 l1) post2)) ==>
-(weak_map_triple m invariant l ls1' (ls2 INTER ls2') pre1 post2)
+(weak_map_triple m invar l ls1 ls2 pre1 post1) ==>
+(!l1 . (l1 IN ls1) ==> (weak_map_triple m invar l1 ls1' ls2' (post1 l1) post2)) ==>
+(weak_map_triple m invar l ls1' (ls2 INTER ls2') pre1 post2)
 ``,
 
 cheat);
@@ -346,9 +344,9 @@ val weak_map_std_seq_comp_thm = prove(``
 (ls1' SUBSET ls2) ==>
 (ls1 INTER ls1' = EMPTY) ==>
 (ls1' INTER ls2' = EMPTY) ==>
-(weak_map_triple m invariant l ls1 ls2 pre1 post1) ==>
-(!l1 . (l1 IN ls1) ==> (weak_map_triple m invariant l1 ls1' ls2' (post1 l1) post2)) ==>
-(weak_map_triple m invariant l ls1' (ls2 INTER ls2') pre1 post2)
+(weak_map_triple m invar l ls1 ls2 pre1 post1) ==>
+(!l1 . (l1 IN ls1) ==> (weak_map_triple m invar l1 ls1' ls2' (post1 l1) post2)) ==>
+(weak_map_triple m invar l ls1' (ls2 INTER ls2') pre1 post2)
 ``,cheat);
 
 
@@ -358,9 +356,9 @@ val weak_map_std_seq_comp_thm = prove(``
 (ls1' SUBSET ls2) ==>
 (ls1 INTER ls1' = EMPTY) ==>
 (ls1' INTER ls2' = EMPTY) ==>
-(weak_map_triple m invariant l ls1 ls2 pre1 post1) ==>
-(!l1 . (l1 IN ls1) ==> (weak_map_triple m invariant l1 ls1' ls2' (post1 l1) post2)) ==>
-(weak_map_triple m invariant l ls1' (ls2 INTER ls2') pre1 post2)
+(weak_map_triple m invar l ls1 ls2 pre1 post1) ==>
+(!l1 . (l1 IN ls1) ==> (weak_map_triple m invar l1 ls1' ls2' (post1 l1) post2)) ==>
+(weak_map_triple m invar l ls1' (ls2 INTER ls2') pre1 post2)
 ``,
 
 cheat);
@@ -372,9 +370,9 @@ val weak_map_std_seq_comp_thm = prove(``
 (ls1' SUBSET ls2) ==>
 (ls1 INTER ls1' = EMPTY) ==>
 (ls1' INTER ls2' = EMPTY) ==>
-(weak_map_triple m invariant l ls1 ls2 pre1 post1) ==>
-(!l1 . (l1 IN ls1) ==> (weak_map_triple m invariant l1 ls1' ls2' (post1 l1) post2)) ==>
-(weak_map_triple m invariant l ls1' (ls2 INTER ls2') pre1 post2)
+(weak_map_triple m invar l ls1 ls2 pre1 post1) ==>
+(!l1 . (l1 IN ls1) ==> (weak_map_triple m invar l1 ls1' ls2' (post1 l1) post2)) ==>
+(weak_map_triple m invar l ls1' (ls2 INTER ls2') pre1 post2)
 ``,
 
 cheat);
@@ -386,9 +384,9 @@ val weak_map_std_seq_comp_thm = prove(``
 (ls1' SUBSET ls2) ==>
 (ls1 INTER ls1' = EMPTY) ==>
 (ls1' INTER ls2' = EMPTY) ==>
-(weak_map_triple m invariant l ls1 ls2 pre1 post1) ==>
-(!l1 . (l1 IN ls1) ==> (weak_map_triple m invariant l1 ls1' ls2' (post1 l1) post2)) ==>
-(weak_map_triple m invariant l ls1' (ls2 INTER ls2') pre1 post2)
+(weak_map_triple m invar l ls1 ls2 pre1 post1) ==>
+(!l1 . (l1 IN ls1) ==> (weak_map_triple m invar l1 ls1' ls2' (post1 l1) post2)) ==>
+(weak_map_triple m invar l ls1' (ls2 INTER ls2') pre1 post2)
 ``,
 
 cheat);
